TangleLearning_Search.thy
@@ -1,6 +1,8 @@
 theory TangleLearning_Search
-imports Main TangleAttractors
+imports Main TangleAttractors TangleLearning
 begin
+
+definition test where "test = finite_graph_V_Succ.nt_bottom_SCC"
 
 context paritygame begin
 
@@ -18,7 +20,7 @@ begin
 
 (** search_step represents a single iteration of the while-loop in the search algorithm. *)
 inductive search_step ::
-  "'v set \<times> ('v set \<times> 'v strat) set \<Rightarrow> 'v set \<times> ('v set \<times> 'v strat) set \<Rightarrow> bool" where
+  "'v set \<times> 'v set  set \<Rightarrow> 'v set \<times> 'v set set \<Rightarrow> bool" where
   step: "\<lbrakk>R \<noteq> {}; R \<subseteq> V; paritygame (Restr E R) (V\<inter>R) (V\<^sub>0\<inter>R);
           p = pr_set R; \<alpha> = player_wins_pr p;
           A = {v. v \<in> R \<and> pr v = p};
@@ -26,30 +28,11 @@ inductive search_step ::
           paritygame.tangle_attractor (Restr E R) (V\<inter>R) (V\<^sub>0\<inter>R) pr \<alpha> T\<^sub>\<alpha> A Z \<sigma>;
           V\<^sub>\<alpha> = V_player \<alpha>; V\<^sub>\<beta> = V_opponent \<alpha>;
           Ov = {v. v \<in> V\<^sub>\<alpha>\<inter>A \<and> E `` {v} \<inter> Z \<noteq> {}} \<union> {v. v \<in> V\<^sub>\<beta>\<inter>A \<and> (E `` {v}) \<inter> R \<subseteq> Z};
-          Y' = (if Ov \<noteq> {} then Y \<union> {(S,\<sigma>). nt_bottom_SCC S} else Y);
+          Y' = (if Ov \<noteq> {} then
+            Y \<union> {S. S \<subseteq> Z \<and> finite_graph_V_Succ.nt_bottom_SCC (induced_subgraph V\<^sub>\<alpha> \<sigma>) (induced_subgraph_V V\<^sub>\<alpha> \<sigma>) S}
+          else
+            Y);
           R' = R-Z\<rbrakk> \<Longrightarrow> search_step (R,Y) (R',Y')"
-
-(** search_step is inversely monotonous on R: R strictly decreases with every step. *)
-lemma search_step_R_anti_mono: "search_step S S' \<Longrightarrow> fst S' \<subset> fst S"
-proof (induction rule: search_step.induct)
-  case (step R p \<alpha> A T\<^sub>\<alpha> Z \<sigma> V\<^sub>\<alpha> V\<^sub>\<beta> Ov Y' Y R')
-  from step(7) have tangles_T\<^sub>\<alpha>: "\<forall>t\<in>T\<^sub>\<alpha>. paritygame.tangle (Restr E R) (V \<inter> R) (V\<^sub>0 \<inter> R) pr \<alpha> t"
-    by blast
-  from step(7) have fin_T\<^sub>\<alpha>: "finite T\<^sub>\<alpha>"
-    using finite_subset[OF _ fin_T] by simp
-
-  from finite_subset[OF step(2) fin_V] have fin_R: "finite R" .
-  from step(1) step(6) step(4) have A_notempty: "A \<noteq> {}"
-    using pr_set_exists[OF fin_R step(1)] by blast
-  from step(6) have A_in_R: "A \<subseteq> R" by simp
-
-  from A_notempty paritygame.target_in_tangle_attractor[OF step(3) tangles_T\<^sub>\<alpha> fin_T\<^sub>\<alpha> step(8)]
-  have Z_notempty: "Z \<noteq> {}" by blast
-  from A_in_R paritygame.tangle_attractor_ss[OF step(3) tangles_T\<^sub>\<alpha> fin_T\<^sub>\<alpha> step(8)] step(2)
-  have Z_in_V_int_R: "Z \<subseteq> V \<inter> R" by blast
-
-  from step(13) Z_notempty Z_in_V_int_R show ?case by auto
-qed
 
 (** If a step can be applied, both R and R' are subsets of V. *)
 lemma search_step_R_in_V: "search_step S S' \<Longrightarrow> fst S \<subseteq> V \<and> fst S' \<subseteq> V"
@@ -58,6 +41,41 @@ lemma search_step_R_in_V: "search_step S S' \<Longrightarrow> fst S \<subseteq> 
 (** If a step can be applied, both R and R' are finite. *)
 lemma search_step_R_finite: "search_step S S' \<Longrightarrow> finite (fst S) \<and> finite (fst S')"
   using search_step_R_in_V finite_subset[OF _ fin_V] by auto
+
+(** search_step is inversely monotonous on R: R strictly decreases with every step. *)
+lemma search_step_R_anti_mono: "search_step S S' \<Longrightarrow> fst S' \<subset> fst S"
+proof (induction rule: search_step.induct)
+  case (step R p \<alpha> A T\<^sub>\<alpha> Z \<sigma> V\<^sub>\<alpha> V\<^sub>\<beta> Ov Y' Y R')
+  (** We know that every t in T\<^sub>\<alpha> is a tangle in the subgame of R, and that T\<^sub>\<alpha> is finite. We need
+      these properties for showing the next two properties. *)
+  from step(7) have tangles_T\<^sub>\<alpha>: "\<forall>t\<in>T\<^sub>\<alpha>. paritygame.tangle (Restr E R) (V \<inter> R) (V\<^sub>0 \<inter> R) pr \<alpha> t"
+    by blast
+  from step(7) have fin_T\<^sub>\<alpha>: "finite T\<^sub>\<alpha>"
+    using finite_subset[OF _ fin_T] by simp
+  (** We show that Z is not empty. *)
+  have "Z \<noteq> {}" proof -
+    (** R is finite *)
+    from finite_subset[OF step(2) fin_V] have fin_R: "finite R" .
+    (** A is part of the finite non-empty set R, therefore, it must contain at least one node
+        with priority p, and thus it is not empty. *)
+    from step(6) step(4) have "A \<noteq> {}"
+      using pr_set_exists[OF fin_R step(1)] by blast
+    (** Since the target A is part of the tangle-attracted region Z, Z must also be non-empty. *)
+    with paritygame.target_in_tangle_attractor[OF step(3) tangles_T\<^sub>\<alpha> fin_T\<^sub>\<alpha> step(8)]
+    show ?thesis by auto
+  qed
+  (** Furthermore, Z is a subset of of R. *)
+  moreover have "Z \<subseteq> R" proof -
+    from step(6) have A_in_R: "A \<subseteq> R" by simp
+    (** Since the tangle-attracted Z region is a subset of the graph restricted to R  and the target
+        set A, we can show that it is a subset R. *)
+    with paritygame.tangle_attractor_ss[OF step(3) tangles_T\<^sub>\<alpha> fin_T\<^sub>\<alpha> step(8)] step(2)
+    show ?thesis by blast
+  qed
+  (** Since R' is obtained by removing Z from R, and we know that Z is a non-empty a subset of R,
+      R decreases monotonically with every step. *)
+  ultimately show ?case using step(13) by auto
+qed
 
 (** Because R is finite and decreases with every step, search_step is a well-founded relation. *)
 lemma search_step_wellfounded: "wfP (search_step\<inverse>\<inverse>)"
@@ -73,15 +91,19 @@ lemma step_result_R_is_paritygame:
   "search_step S S' \<Longrightarrow> paritygame (Restr E (fst S')) (V\<inter>fst S') (V\<^sub>0\<inter>fst S')"
 proof (induction rule: search_step.induct)
   case (step R p \<alpha> A T\<^sub>\<alpha> Z \<sigma> V\<^sub>\<alpha> V\<^sub>\<beta> Ov Y' Y R')
-
+  (** We know that every tangle t in T\<^sub>\<alpha> is a tangle in the subgame of R, and that T\<^sub>\<alpha> is finite. *)
   from step(7) have tangles_T\<^sub>\<alpha>: "\<forall>t\<in>T\<^sub>\<alpha>. paritygame.tangle (Restr E R) (V \<inter> R) (V\<^sub>0 \<inter> R) pr \<alpha> t"
     by simp
   from step(7) have fin_T\<^sub>\<alpha>: "finite T\<^sub>\<alpha>"
     using finite_subset[OF _ fin_T] by simp
-
+  (** We can write any instance of R-Z as R'. *)
   from step(13) have "(V \<inter> R-Z) = (V \<inter> R')" by blast
   moreover from step(13) have "(V\<^sub>0 \<inter> R-Z) = (V\<^sub>0 \<inter> R')" by blast
+  (** If we restrict the already restricted graph R to R', we find that it is the same as
+      restricting the whole graph to R'. *)
   moreover from step(13) have "(Restr (Restr E R) (V \<inter> R')) = Restr E R'" using E_in_V by auto
+  (** Now, we can show that removing the tangle-attracted region from the graph yields a valid
+      subgame. *)
   ultimately show ?case
     using paritygame.remove_tangle_attractor_subgame[OF step(3) tangles_T\<^sub>\<alpha> fin_T\<^sub>\<alpha> step(8)] by auto
 qed
@@ -110,26 +132,16 @@ proof -
   moreover define V\<^sub>\<beta> where "V\<^sub>\<beta> = V_opponent \<alpha>"
   moreover define Ov where
     "Ov = {v. v \<in> V\<^sub>\<alpha>\<inter>A \<and> E `` {v} \<inter> Z \<noteq> {}} \<union> {v. v \<in> V\<^sub>\<beta>\<inter>A \<and> (E `` {v}) \<inter> R \<subseteq> Z}"
-  moreover define Y' where "Y' = (if Ov \<noteq> {} then Y \<union> {(S,\<sigma>). nt_bottom_SCC S} else Y)"
+  moreover define Y' where "Y' = (if Ov \<noteq> {} then
+      Y \<union> {S. S \<subseteq> Z \<and> finite_graph_V_Succ.nt_bottom_SCC (induced_subgraph V\<^sub>\<alpha> \<sigma>) (induced_subgraph_V V\<^sub>\<alpha> \<sigma>) S}
+   else
+      Y)"
   moreover define R' where "R' = R-Z"
   (** Now, we can put them in their place in the step, and our thesis follows automatically. *)
   ultimately have "search_step (R,Y) (R',Y')"
     using search_step.step by blast
   thus ?thesis by blast
 qed
-
-(** TODO: invariant, prove property of Y on termination. *)
-
-(** The search algorithm applies the search_step until it reaches the end.
-    We do not have to specify that ({},Y) is not in the domain of the step,
-    as this follows automatically because an empty R is not allowed.
-    (see next lemma) *)
-definition search :: "'v set \<Rightarrow> ('v set \<times> 'v strat) set \<Rightarrow> bool" where
-  "search R Y \<equiv> search_step\<^sup>*\<^sup>* (R,{}) ({},Y)"
-
-lemma search_terminates_on_empty_R: "\<not>Domainp search_step ({},Y)"
-  using search_step_R_anti_mono[of "({},Y)"]
-  by auto
 
 (** If we start from a valid, non-empty subgame, through applying search_step, we will always reach
     a final state with a corresponding Y. *)
@@ -172,6 +184,172 @@ proof (induction S rule: wf_induct_rule)
   qed
 qed
 
+(** When an empty R is reached, there exist no further steps in the algorithm. *)
+lemma search_terminates_on_empty_R: "\<not>Domainp search_step ({},Y)"
+  using search_step_R_anti_mono[of "({},Y)"]
+  by auto
+
+lemma "search_step S S' \<Longrightarrow> snd S \<subseteq> snd S'"
+  apply (induction rule: search_step.induct) by auto
+
+(** TODO: invariant, prove property of Y on termination. *)
+(** The current invariant states that everything contained in Y is a tangle.
+    This should probably be restated to say that everything contained in Y is a tangle with its
+    corresponding strategy. *)
+definition search_I ::  "'v set \<times> 'v set set \<Rightarrow> bool" where
+  "search_I S \<equiv> finite (snd S) \<and> (\<forall>U \<in> snd S. \<exists>\<alpha>. tangle \<alpha> U)"
+
+lemma search_step_preserves_I:
+  "search_step S S' \<Longrightarrow> search_I S \<Longrightarrow> search_I S'"
+proof (induction rule: search_step.induct)
+  case (step R p \<alpha> A T\<^sub>\<alpha> Z \<sigma> V\<^sub>\<alpha> V\<^sub>\<beta> Ov Y' Y R')
+  (** We know that every tangle t in T\<^sub>\<alpha> is a tangle in the subgame of R, and that T\<^sub>\<alpha> is finite. *)
+  from step(7) have tangles_T\<^sub>\<alpha>: "\<forall>t\<in>T\<^sub>\<alpha>. paritygame.tangle (Restr E R) (V \<inter> R) (V\<^sub>0 \<inter> R) pr \<alpha> t"
+    by simp
+  from step(7) have fin_T\<^sub>\<alpha>: "finite T\<^sub>\<alpha>"
+    using finite_subset[OF _ fin_T] by simp
+
+  from step(2,4,5) have player_wins_R: "player_winningP \<alpha> (pr_set (V \<inter> R))"
+    unfolding player_wins_pr_def
+    by (simp split: if_splits add: Int_absorb1)
+
+  from step(2,4,6) have A': "A = {v \<in> V \<inter> R. pr v = pr_set (V \<inter> R)}"
+    by (simp add: Int_absorb1)
+
+  from paritygame.target_in_tangle_attractor[OF step(3) tangles_T\<^sub>\<alpha> fin_T\<^sub>\<alpha> step(8)]
+       paritygame.tangle_attractor_ss[OF step(3) tangles_T\<^sub>\<alpha> fin_T\<^sub>\<alpha> step(8)] step(2,6)
+  have A_in_Z: "A \<subseteq> Z" and Z_in_R: "Z \<subseteq> R" by blast+
+
+  have "paritygame.strategy_of_player (Restr E R) (V\<inter>R) (V\<^sub>0\<inter>R) \<alpha> \<sigma> = strategy_of_player \<alpha> \<sigma>"
+    unfolding paritygame.strategy_of_player_def[OF step(3)] strategy_of_player_def
+    unfolding arena.strategy_of_def[OF paritygame.axioms[OF step(3)]] strategy_of_def
+    unfolding restr_subgraph_V_player[OF step(3)]
+    unfolding E_of_strat_def
+    apply (cases \<alpha>; clarsimp simp add: V\<^sub>1_def)
+    xxx, sorry
+
+  from Z_in_R paritygame.tangle_attractor_strat[OF step(3) tangles_T\<^sub>\<alpha> fin_T\<^sub>\<alpha> step(8)] 
+       restr_subgraph_V_player[OF step(3)] restr_ind_subgraph_V\<^sub>\<alpha>[OF paritygame.axioms[OF step(3)]]
+  have
+    \<sigma>_strat: "paritygame.strategy_of_player (Restr E R) (V\<inter>R) (V\<^sub>0\<inter>R) \<alpha> \<sigma>" and
+    \<sigma>_dom: "dom \<sigma> = V_player \<alpha> \<inter> (Z-A)" and
+    \<sigma>_ran: "ran \<sigma> \<subseteq> Z" and
+    \<sigma>_closed_opp: "Restr (induced_subgraph (V_player \<alpha>) \<sigma>) R `` (Z-A) \<subseteq> Z" and
+    \<sigma>_forces_A_or_wins: "\<forall>x\<in>Z. \<forall>xs ys.
+      lasso_from_node (Restr (induced_subgraph (V_player \<alpha>) \<sigma>) R) x xs ys
+        \<longrightarrow> set (xs @ ys) \<inter> A \<noteq> {} \<or> player_wins_list \<alpha> ys"
+    by auto
+   
+
+  have "\<forall>v\<in>Z. \<forall>xs ys. lasso_from_node (Restr (induced_subgraph (V_player \<alpha>) \<sigma>) Z) v xs ys
+          \<longrightarrow> player_wins_list \<alpha> ys"
+  proof (rule ballI; intro allI; rule impI)
+    fix v xs ys
+    assume v_in_Z: "v \<in> Z" and
+      lasso_v_xs_ys: "lasso_from_node (Restr (induced_subgraph (V_player \<alpha>) \<sigma>) Z) v xs ys"
+
+    (** This should be a lemma. *)
+    from \<open>Z\<subseteq>R\<close> have "(Restr (induced_subgraph (V_player \<alpha>) \<sigma>) Z) \<subseteq>
+            (Restr (arena.induced_subgraph (Restr E R) (paritygame.V_player (V\<inter>R) (V\<^sub>0\<inter>R) \<alpha>) \<sigma>) Z)"
+      unfolding arena.induced_subgraph_def[OF paritygame.axioms[OF step(3)]] induced_subgraph_def
+      using paritygame.V_player.simps[OF step(3)]
+      by (cases \<alpha>; auto simp: V\<^sub>1_def arena.V\<^sub>1_def[OF paritygame.axioms[OF step(3)]])
+
+    from paritygame.van_dijk_2[OF step(3) tangles_T\<^sub>\<alpha> fin_T\<^sub>\<alpha> player_wins_R A' step(8)]
+      v_in_Z subgraph_lasso[OF this lasso_v_xs_ys]
+    show "player_wins_list \<alpha> ys" by blast
+  qed
+
+  from step.prems have
+    fin_Y: "finite Y" and
+    tangles_Y: "\<forall>U \<in> Y. \<exists>\<alpha>. tangle \<alpha> U"
+    unfolding search_I_def
+    by auto
+
+  show ?case
+    unfolding search_I_def
+  proof (intro conjI)
+    from finite_subset[OF Z_in_R finite_subset[OF step(2) fin_V]]
+    have fin_Z: "finite Z" .
+    hence fin_Y'_additions:
+      "finite {S. S \<subseteq> Z \<and> finite_graph_V_Succ.nt_bottom_SCC (induced_subgraph V\<^sub>\<alpha> \<sigma>) (induced_subgraph_V V\<^sub>\<alpha> \<sigma>) S}"
+    by simp
+    with fin_Y step(12) show "finite (snd (R',Y'))" by simp
+  next
+    show "\<forall>U\<in>snd (R', Y'). \<exists>\<alpha>. tangle \<alpha> U"
+    proof (rule ballI; clarsimp)
+      fix U
+      assume U_in_Y': "U \<in> Y'"
+      with step(12) consider
+        (old) "U \<in> Y"
+      | (new) "U \<in> {S. S \<subseteq> Z \<and> finite_graph_V_Succ.nt_bottom_SCC (induced_subgraph V\<^sub>\<alpha> \<sigma>) (induced_subgraph_V V\<^sub>\<alpha> \<sigma>) S}"
+        by (auto split: if_splits)
+      thus "\<exists>\<alpha>. tangle \<alpha> U" proof cases
+        case old with tangles_Y show ?thesis by blast
+      next
+        case new
+        hence U_in_Z: "U\<subseteq>Z" and
+          SCC_U: "finite_graph_V_Succ.nt_bottom_SCC (induced_subgraph V\<^sub>\<alpha> \<sigma>) (induced_subgraph_V V\<^sub>\<alpha> \<sigma>) U"
+          by auto
+
+        (** This should be a lemma. In fact, there is a similar lemma, but it is limited to
+            V\<^sub>\<alpha> = dom \<sigma>, which is not the case here. *)
+        have "finite_graph_V_Succ (induced_subgraph V\<^sub>\<alpha> \<sigma>) (induced_subgraph_V V\<^sub>\<alpha> \<sigma>)"
+        proof (unfold_locales)
+          show "induced_subgraph V\<^sub>\<alpha> \<sigma> \<subseteq> induced_subgraph_V V\<^sub>\<alpha> \<sigma> \<times> induced_subgraph_V V\<^sub>\<alpha> \<sigma>"
+            unfolding induced_subgraph_V_def by force
+        next
+          show "finite (induced_subgraph_V V\<^sub>\<alpha> \<sigma>)" by simp
+        next
+          show "\<And>v. v \<in> induced_subgraph_V V\<^sub>\<alpha> \<sigma> \<Longrightarrow> induced_subgraph V\<^sub>\<alpha> \<sigma> `` {v} \<noteq> {}"
+          proof -
+            fix v
+            assume v_in_subgraph: "v \<in> induced_subgraph_V V\<^sub>\<alpha> \<sigma>"
+            from paritygame.player_strat_in_E[OF step(3) \<sigma>_strat]
+            have \<sigma>_edges_in_E: "E_of_strat \<sigma> \<subseteq> E" by simp
+
+            consider (dom) "v \<in> dom \<sigma>" | (not_dom) "v \<notin> dom \<sigma>" by blast
+            thus "induced_subgraph V\<^sub>\<alpha> \<sigma> `` {v} \<noteq> {}" proof cases
+              case dom with \<sigma>_edges_in_E show ?thesis
+                using edge_in_E_of_strat[of \<sigma>] strategy_to_ind_subgraph by blast
+            next
+              case not_dom
+              from v_in_subgraph have "v \<in> V" using ind_subgraph_V_in_V by blast
+              then obtain v' where "(v,v') \<in> E" using succ by blast
+              consider (in_V\<^sub>\<alpha>) "v \<in> V\<^sub>\<alpha>" | (notin_V\<^sub>\<alpha>) "v \<notin> V\<^sub>\<alpha>" by blast
+              thus ?thesis proof cases
+                case in_V\<^sub>\<alpha>
+                with Z_in_R not_dom have "v \<notin> (Z-A)"
+                  unfolding step(9) \<sigma>_dom by blast
+                show ?thesis sorry
+              next
+                case notin_V\<^sub>\<alpha>
+                from ind_subgraph_notin_dom[OF \<open>(v,v')\<in>E\<close> notin_V\<^sub>\<alpha>]
+                show ?thesis by blast
+              qed
+            qed
+          qed
+        qed
+        have "U \<noteq> {}" sorry
+
+        
+        show ?thesis
+          unfolding tangle_iff tangle_strat_iff sorry
+      qed
+    qed
+  qed
+qed
+
+lemma search_step_rtranclp_preserves_I:
+  "search_step\<^sup>*\<^sup>* S S' \<Longrightarrow> search_I S \<Longrightarrow> search_I S'"
+  apply (induction rule: rtranclp_induct)
+  using search_step_preserves_I by auto
+
+(** The search algorithm applies the search_step until it reaches the end.
+    We do not have to specify that ({},Y) is not in the domain of the step,
+    as this follows automatically because no further steps exist from an empty R. *)
+definition search :: "'v set \<Rightarrow> 'v set set \<Rightarrow> bool" where
+  "search R Y \<equiv> search_step\<^sup>*\<^sup>* (R,{}) ({},Y)"
 
 (** For every valid, non-empty subgame R, the search algorithm finds a Y. *)
 lemma search_has_result:
@@ -179,6 +357,21 @@ lemma search_has_result:
   unfolding search_def
   using search_step_terminates_with_Y by simp
 
+lemma search_preserves_I:
+  "search R Y \<Longrightarrow> search_I ({},Y)"
+  unfolding search_def
+  apply (induction rule: rtranclp_induct)
+  subgoal unfolding search_I_def by simp
+  subgoal using search_step_rtranclp_preserves_I by blast
+  done
+
+lemma search_finds_tangles:
+  shows "search R Y \<Longrightarrow> Y \<noteq> {} \<and> finite Y \<and> (\<forall>U \<in> Y. \<exists>\<alpha>. tangle \<alpha> U)"
+  apply (intro conjI)
+  subgoal sorry
+  subgoal using search_preserves_I unfolding search_I_def by simp
+  subgoal using search_preserves_I unfolding search_I_def by simp
+  done
 end (** End of context with fixed T. *)
 
 end (** End of context paritygame *)
