StrongConnectivity.thy
@@ -252,6 +252,18 @@ definition nt_bottom_SCC :: "'v set \<Rightarrow> bool" where
 lemma nt_bottom_SCC_is_bottom_SCC:
   "nt_bottom_SCC R \<Longrightarrow> bottom_SCC R"
   unfolding nt_bottom_SCC_def by simp
+
+lemma finite_SCCs:
+  "finite {R. SCC R}"
+  unfolding SCC_def by fast
+
+lemma finite_bottom_SCCs:
+  "finite {R. bottom_SCC R}"
+  using finite_subset[OF Collect_mono finite_SCCs] bottom_SCC_is_SCC by blast
+
+lemma finite_nt_bottom_SCCs: 
+  "finite {R. nt_bottom_SCC R}"
+  using finite_subset[OF Collect_mono finite_bottom_SCCs] nt_bottom_SCC_is_bottom_SCC by blast
 end (** End of context finite_graph_V_Succ *)
 
 end
